More work in connecting instances of operational semantics to their type classes.

HoareLogic/BigStepSemantics.v
@@ -43,28 +43,27 @@ Class SABigStepSemantics (P: ProgrammingLanguage) (state: Type) {J: Join state} 
   frame_property: forall m mf m' c n', join m mf m' -> access m' c n' -> exists n nf, Korder nf mf /\ lift_join n (Terminating nf) n' /\ access m c n
 }.
 
+Module ImpBigStepSemantics (D: DECREASE).
+
+Export D.
+
 Inductive loop_access_fin
           {state: Type}
           {kiM: KripkeIntuitionisticModel state}
           (R: state -> MetaState state -> Prop)
           (test: state -> Prop): state -> MetaState state -> Prop :=
 | loop_access_Terminating:
-    forall s1 s2,
+    forall s1 ms2,
       ~ test s1 ->
-      Korder s2 s1 ->
-      loop_access_fin R test s1 (Terminating s2)
-| loop_access_Error:
-    forall s1 s2,
+      decrease (Terminating s1) ms2 ->
+      loop_access_fin R test s1 ms2
+| loop_access_abnormal:
+    forall s1 ms2 ms3,
       test s1 ->
-      Korder s2 s1 ->
-      R s2 Error ->
-      loop_access_fin R test s1 Error
-| loop_access_fin_NonTerminating:
-    forall s1 s2,
-      test s1 ->
-      Korder s2 s1 ->
-      R s2 NonTerminating ->
-      loop_access_fin R test s1 NonTerminating
+      decrease (Terminating s1) ms2 ->
+      lift_relation R ms2 ms3 ->
+      ms3 = Error \/ ms3 = NonTerminating ->
+      loop_access_fin R test s1 ms3
 | loop_access_step:
     forall s1 s2 s3 s4 ms,
       test s1 ->
@@ -87,70 +86,56 @@ Inductive loop_access_inf
       (forall n, Korder (s1 (S n)) (s3 n)) ->
       loop_access_inf R test (s1 0).
 
-Inductive loop_access
-          {state: Type}
-          {kiM: KripkeIntuitionisticModel state}
-          (R: state -> MetaState state -> Prop)
-          (test: state -> Prop): state -> MetaState state -> Prop :=
-| loop_access_loop_access_fin:
-    forall s ms, loop_access_fin R test s ms ->
-      loop_access R test s ms
-| loop_access_loop_access_inf:
-    forall s, loop_access_inf R test s ->
-      loop_access R test s NonTerminating.
-
-Module Total.
-
 Class ImpBigStepSemantics (P: ProgrammingLanguage) {iP: ImperativeProgrammingLanguage P} (state: Type) {kiM: KripkeIntuitionisticModel state} (BSS: BigStepSemantics P state): Type := {
   eval_bool: state -> bool_expr -> Prop;
   eval_bool_stable: forall b, Korder_stable (fun s => eval_bool s b);
   access_Ssequence: forall c1 c2 s ms,
     access s (Ssequence c1 c2) ms ->
     exists ms' ms'',
-      access s c1 ms' /\ lift_Korder ms'' ms' /\ lift_access ms'' c2 ms;
+      access s c1 ms' /\ decrease ms' ms'' /\ lift_access ms'' c2 ms;
   access_Sifthenelse: forall b c1 c2 s ms,
     access s (Sifthenelse b c1 c2) ms ->
-    (eval_bool s b /\ exists s', Korder s' s /\ access s' c1 ms) \/
-    (~ eval_bool s b /\ exists s', Korder s' s /\ access s' c2 ms);
+    (eval_bool s b /\ exists ms', decrease (Terminating s) ms' /\ lift_access ms' c1 ms) \/
+    (~ eval_bool s b /\ exists ms', decrease (Terminating s) ms' /\ lift_access ms' c2 ms);
   access_Swhile: forall b c s ms,
     access s (Swhile b c) ms ->
-    loop_access (fun s ms => access s c ms) (fun s => eval_bool s b) s ms
+    (loop_access_fin (fun s ms => access s c ms) (fun s => eval_bool s b) s ms) \/
+    (loop_access_inf (fun s ms => access s c ms) (fun s => eval_bool s b) s /\ ms = NonTerminating)
 }.
 
-End Total.
+End ImpBigStepSemantics.
 
-Module Partial.
+Module Total := ImpBigStepSemantics (ProgramState.Total).
 
-Class ImpBigStepSemantics (P: ProgrammingLanguage) {iP: ImperativeProgrammingLanguage P} (state: Type) {kiM: KripkeIntuitionisticModel state} (BSS: BigStepSemantics P state): Type := {
-  eval_bool: state -> bool_expr -> Prop;
-  eval_bool_stable: forall b, Korder_stable (fun s => eval_bool s b);
-  access_Ssequence: forall c1 c2 s ms,
-    access s (Ssequence c1 c2) ms ->
-    exists ms' ms'',
-      access s c1 ms' /\ lift_Korder ms'' ms' /\ lift_access ms'' c2 ms;
-  access_Sifthenelse: forall b c1 c2 s ms,
-    access s (Sifthenelse b c1 c2) ms ->
-    ms = NonTerminating \/
-    (eval_bool s b /\ exists s', Korder s' s /\ access s' c1 ms) \/
-    (~ eval_bool s b /\ exists s', Korder s' s /\ access s' c2 ms);
-  access_Swhile: forall b c s ms,
-    access s (Swhile b c) ms ->
-    ms = NonTerminating \/
-    loop_access_fin (fun s ms => access s c ms) (fun s => eval_bool s b) s ms
-}.
-
-End Partial.
+Module Partial := ImpBigStepSemantics (ProgramState.Partial).
 
 Instance Total2Partial_ImpBigStepSemantics {P: ProgrammingLanguage} {iP: ImperativeProgrammingLanguage P} (state: Type) {kiM: KripkeIntuitionisticModel state} {BSS: BigStepSemantics P state} (iBSS: Total.ImpBigStepSemantics P state BSS): Partial.ImpBigStepSemantics P state BSS.
 Proof.
   refine (Partial.Build_ImpBigStepSemantics _ _ _ _ _ Total.eval_bool Total.eval_bool_stable _ _ _).
-  + apply Total.access_Ssequence.
   + intros.
-    pose proof Total.access_Sifthenelse b c1 c2 s ms H.
-    tauto.
+    pose proof Total.access_Ssequence c1 c2 s ms H
+      as [ms' [ms'' [? [? ?]]]].
+    exists ms', ms''; split; [| split]; auto.
+    apply Total2Partial_decrease; auto.
+  + intros.
+    pose proof Total.access_Sifthenelse b c1 c2 s ms H
+      as [[? [ms' [? ?]]] | [? [ms' [? ?]]]].
+    - left; split; auto; exists ms'; split; auto.
+      apply Total2Partial_decrease; auto.
+    - right; split; auto; exists ms'; split; auto.
+      apply Total2Partial_decrease; auto.
   + intros.
     pose proof Total.access_Swhile b c s ms H.
-    destruct H0; tauto.
+    destruct H0 as [? | [? ?]].
+    - left.
+      clear H; induction H0.
+      * apply Partial.loop_access_Terminating; auto.
+        apply Total2Partial_decrease; auto.
+      * eapply Partial.loop_access_abnormal; eauto.
+        apply Total2Partial_decrease; auto.
+      * apply (Partial.loop_access_step _ _ s1 s2 s3 s4); eauto.
+    - right; split; auto.
+      clear ms H1 H.
+      inversion H0; subst.
+      econstructor; eauto.
 Defined.
-
-
