HoareLogic/ImperativeLanguage.v
@@ -24,3 +24,14 @@ Class Lock_ConcurrentProgrammingLanguage (P: ProgrammingLanguage): Type := {
   Sacquire: lock_expr -> cmd;
   Srelease: lock_expr -> cmd
 }.
+
+Class NormalImperativeProgrammingLanguage (P: ProgrammingLanguage) {iP: ImperativeProgrammingLanguage P}: Type := {
+  Ssequence_inv: forall c1 c2 c1' c2', Ssequence c1 c2 = Ssequence c1' c2' -> c1 = c1' /\ c2 = c2';
+  Ssequence_Sskip: forall c1 c2, Ssequence c1 c2 <> Sskip;
+  Sifthenelse_inv: forall b c1 c2 b' c1' c2', Sifthenelse b c1 c2 = Sifthenelse b' c1' c2' -> b = b' /\ c1 = c1' /\ c2 = c2';
+  Sifthenelse_Sskip: forall b c1 c2, Sifthenelse b c1 c2 <> Sskip;
+  Swhile_inv: forall b c b' c', Swhile b c = Swhile b' c' -> b = b' /\ c = c';
+  Swhile_Sskip: forall b c, Swhile b c <> Sskip
+}.
+
+
