HoareLogic/SmallStepSemantics.v
@@ -45,47 +45,58 @@ Class SASmallStepSemantics (P: ProgrammingLanguage) (state: Type) {J: Join state
   frame_property: forall (m mf m': cmd * state) n', join (snd m) (snd mf) (snd m') -> step_safe m -> step m' n' -> exists n nf, Korder (snd nf) (snd mf) /\ @lift_join _ (@prod_Join cmd state (equiv_Join cmd) J) n (Terminating nf) n' /\ step m n
 }.
 
-Module Partial.
+Module ImpSmallStepSemantics (D: DECREASE).
+
+Export D.
 
 Class ImpSmallStepSemantics (P: ProgrammingLanguage) {iP: ImperativeProgrammingLanguage P} (state: Type) {kiM: KripkeIntuitionisticModel state} (SSS: SmallStepSemantics P state): Type := {
   eval_bool: state -> bool_expr -> Prop;
   eval_bool_stable: forall b, Korder_stable (fun s => eval_bool s b);
   step_Ssequence: forall c1 c2 s mcs,
     step (Ssequence c1 c2, s) mcs ->
-    mcs = NonTerminating \/
-    (exists s', c1 = Sskip /\ Korder s' s /\ mcs = Terminating (c2, s')) \/
+    (exists ms', c1 = Sskip /\ decrease (Terminating s) ms' /\ mcs = lift_function (pair c2) ms') \/
     (exists mcs', step (c2, s) mcs' /\ mcs = lift_function (fun cs => (Ssequence c1 (fst cs), snd cs)) mcs');
   step_Sifthenelse: forall b c1 c2 s mcs,
     step (Sifthenelse b c1 c2, s) mcs ->
-    mcs = NonTerminating \/
-    (eval_bool s b /\ exists s', Korder s' s /\ mcs = Terminating (c1, s')) \/
-    (~ eval_bool s b /\ exists s', Korder s' s /\ mcs = Terminating (c2, s'));
+    (eval_bool s b /\ exists ms', decrease (Terminating s) ms' /\ mcs = lift_function (pair c1) ms') \/
+    (~ eval_bool s b /\ exists ms', decrease (Terminating s) ms' /\ mcs = lift_function (pair c2) ms');
   step_Swhile: forall b c s mcs,
     step (Swhile b c, s) mcs ->
-    mcs = NonTerminating \/
-    (eval_bool s b /\ exists s', Korder s' s /\ mcs = Terminating (Ssequence c (Swhile b c), s')) \/
-    (~ eval_bool s b /\ exists s', Korder s' s /\ mcs = Terminating (Sskip, s'))
+    (eval_bool s b /\ exists ms', decrease (Terminating s) ms' /\ mcs = lift_function (pair (Ssequence c (Swhile b c))) ms') \/
+    (~ eval_bool s b /\ exists ms', decrease (Terminating s) ms' /\ mcs = lift_function (pair Sskip) ms')
 }.
 
-End Partial.
+End ImpSmallStepSemantics.
 
-Module Total.
+Module Partial := ImpSmallStepSemantics (ProgramState.Partial).
 
-Class ImpSmallStepSemantics (P: ProgrammingLanguage) {iP: ImperativeProgrammingLanguage P} (state: Type) {kiM: KripkeIntuitionisticModel state} (SSS: SmallStepSemantics P state): Type := {
-  eval_bool: state -> bool_expr -> Prop;
-  eval_bool_stable: forall b, Korder_stable (fun s => eval_bool s b);
-  step_Ssequence: forall c1 c2 s mcs,
-    step (Ssequence c1 c2, s) mcs ->
-    (exists s', c1 = Sskip /\ Korder s' s /\ mcs = Terminating (c2, s')) \/
-    (exists mcs', step (c2, s) mcs' /\ mcs = lift_function (fun cs => (Ssequence c1 (fst cs), snd cs)) mcs');
-  step_Sifthenelse: forall b c1 c2 s mcs,
-    step (Sifthenelse b c1 c2, s) mcs ->
-    (eval_bool s b /\ exists s', Korder s' s /\ mcs = Terminating (c1, s')) \/
-    (~ eval_bool s b /\ exists s', Korder s' s /\ mcs = Terminating (c2, s'));
-  step_Swhile: forall b c s mcs,
-    step (Swhile b c, s) mcs ->
-    (eval_bool s b /\ exists s', Korder s' s /\ mcs = Terminating (Ssequence c (Swhile b c), s')) \/
-    (~ eval_bool s b /\ exists s', Korder s' s /\ mcs = Terminating (Sskip, s'))
-}.
+Module Total := ImpSmallStepSemantics (ProgramState.Total).
 
-End Total.
+Instance Total2Partial_ImpSmallStepSemantics {P: ProgrammingLanguage} {iP: ImperativeProgrammingLanguage P} (state: Type) {kiM: KripkeIntuitionisticModel state} {SSS: SmallStepSemantics P state} (iSSS: Total.ImpSmallStepSemantics P state SSS): Partial.ImpSmallStepSemantics P state SSS.
+Proof.
+  refine (Partial.Build_ImpSmallStepSemantics _ _ _ _ _ Total.eval_bool Total.eval_bool_stable _ _ _).
+  + intros.
+    pose proof Total.step_Ssequence c1 c2 s mcs H
+      as [[ms' [? [? ?]]] | [ms' [? ?]]].
+    - left; exists ms'; split; [| split]; auto.
+      apply Total2Partial_decrease; auto.
+    - right; exists ms'; auto.
+  + intros.
+    pose proof Total.step_Sifthenelse b c1 c2 s mcs H
+      as [[? [ms' [? ?]]] | [? [ms' [? ?]]]].
+    - left; split; auto.
+      exists ms'; split; auto.
+      apply Total2Partial_decrease; auto.
+    - right; split; auto.
+      exists ms'; split; auto.
+      apply Total2Partial_decrease; auto.
+  + intros.
+    pose proof Total.step_Swhile b c s mcs H
+      as [[? [ms' [? ?]]] | [? [ms' [? ?]]]].
+    - left; split; auto.
+      exists ms'; split; auto.
+      apply Total2Partial_decrease; auto.
+    - right; split; auto.
+      exists ms'; split; auto.
+      apply Total2Partial_decrease; auto.
+Qed.
